New case analysis scheme for ctx.In and cleanup of ctx.In views

theories/Context.v
@@ -159,58 +159,189 @@ Module Import ctx.
 
     End WithUIP.
 
-    Section In.
-      (* Set locally only for the definition of In. *)
-      Local Set Primitive Projections.
+    (* Definition of context membership proofs [In] for a well-typed de Bruijn
+       representation. Ideally, we would represent [In] inductively using
 
-       (* InCtx represents context containment proofs. This is essentially a
-          well-typed de Bruijn index, i.e. a de Bruijn index with a proof that it
-          resolves to the binding b. This record type is defined using primitive
-          projections to get eta-conversion definitionally. *)
-      Class In (b : B) (Γ : Ctx B) : Set :=
-        MkIn
-          { in_at: nat;
-            in_valid: nth_is Γ in_at b
-          }.
+         Inductive In : B -> Ctx B -> Set :=
+         | in_zero {b Γ}                   : In b (snoc Γ b)
+         | in_succ {b Γ b'} (bIn : In b Γ) : In b (snoc Γ b').
 
-      Global Arguments MkIn [_ _] _ _.
-      Global Arguments in_at [_ _] _.
-      Global Arguments in_valid [_ _] _.
+       However, this representation is not very efficient. Instead, we represent
+       the de Bruijn index using an ordinary natural combined with a proof
+       witness, i.e. a proof that the n-th element in the context from the right
+       is the correct one. We package everything up in a record which is defined
+       as a typeclass to automatically insert proofs (and to give us hooks to
+       define name-based variable resolution later). Furthermore, the record
+       (class) is defined using primitive projections to get eta-equality
+       definitionally. We try to mimick the above inductive definition as much
+       as possible and define case analysis and elimination schemes for the
+       record that coincide with the ones that would be derived for the
+       inductive type. *)
+    #[projections(primitive)]
+    Class In (b : B) (Γ : Ctx B) : Set :=
+      MkIn { in_at: nat; in_valid: nth_is Γ in_at b }.
+    #[global] Arguments MkIn [_ _] _ _.
+    #[global] Arguments in_at [_ _] _.
+    #[global] Arguments in_valid [_ _] _.
 
-      #[program] Instance NoConfusionPackage_In {uip_B : UIP B} {b Γ} : NoConfusionPackage (In b Γ) :=
-         {| NoConfusion xIn yIn := NoConfusion (in_at xIn) (in_at yIn);
-            noConfusion xIn yIn (e : NoConfusion (in_at xIn) (in_at yIn)) :=
-              match noConfusion e in _ = y
-                return forall q, xIn = {| in_at := y; in_valid := q |}
-              with
-              | eq_refl => fun q => f_equal (MkIn _) (proof_irrelevance_nth_is _ _ (in_valid xIn) q)
-              end (in_valid yIn);
-            noConfusion_inv (xIn yIn : In b Γ) (e : xIn = yIn) :=
-              noConfusion_inv (f_equal (@in_at b Γ) e);
-         |}.
-      Next Obligation.
-        intros ? ? ? [m p] [n q] e. cbn [in_at] in *.
-        change (NoConfusion _ _) with (NoConfusion m n) in e.
-        destruct (noConfusion e) eqn:?. cbn.
-        destruct (proof_irrelevance_nth_is m b p q). cbn.
-        destruct m.
-        - destruct e. reflexivity.
-        - apply uip.
-      Qed.
-      Next Obligation.
-        intros ? ? ? [m p] [n q] e; intros.
-        destruct e.
-        destruct Γ; cbn in *. contradiction.
-        destruct m, n.
-        - destruct p. cbn. now rewrite EqDec.uip_refl_refl.
-        - destruct p. cbn. now rewrite EqDec.uip_refl_refl.
-        - cbn. rewrite proof_irrelevance_nth_is_refl. reflexivity.
-        - cbn. rewrite proof_irrelevance_nth_is_refl. reflexivity.
-      Qed.
+    (* These are smart *constructors* for In. *)
+    Definition in_zero {b : B} {Γ : Ctx B} : In b (snoc Γ b) :=
+      @MkIn _ (snoc Γ b) 0 eq_refl.
+    Definition in_succ {b : B} {Γ : Ctx B} {b' : B} (bIn : In b Γ) :
+      In b (snoc Γ b') :=
+      @MkIn _ (snoc Γ b') (S (in_at bIn)) (in_valid bIn).
 
-    End In.
+    (* A case analysis scheme for [In]. This corresponds to a pattern match on
+       the constructors. This case analysis scheme can be used to write function
+       that appear to recurse over an [In] value. Coq's termination checker will
+       inspect this scheme and see the pattern match on the context. This means,
+       that in principle Coq should recognize recursive functions over
+       membership witnesses implemented using this analysis scheme as being
+       structurally recursive (in the context argument). *)
+    Definition In_case (P : forall (b : B) (Γ : Ctx B), In b Γ -> Type)
+      (fz : forall b Γ, P b (snoc Γ b) in_zero)
+      (fs : forall b' Γ b bIn, P b (snoc Γ b') (in_succ bIn)) :
+      forall [b Γ] i, P b Γ i :=
+      fun b Γ =>
+       match Γ with
+       | nil       => fun i => match @in_valid _ _ i with end
+       | snoc Γ b' =>
+           fun '(MkIn n p) =>
+             match n return forall p : nth_is (snoc Γ b') n b, P _ _ (MkIn n p)
+             with
+             | O   => fun 'eq_refl => fz b' Γ
+             | S n => fun p => fs _ _ _ (MkIn n p)
+             end p
+       end.
 
-    (* Two proofs of context containment are equal of the deBruijn indices are equal *)
+    (* Manually define a recursive elimination scheme for [In] using the case
+       analysis scheme above. *)
+    Definition In_rect (P : forall b Γ, In b Γ -> Type)
+      (fz : forall b Γ, P b (snoc Γ b) in_zero)
+      (fs : forall b Γ b' bIn, P b Γ bIn -> P b (snoc Γ b') (in_succ bIn)) :
+      forall b Γ bIn, P b Γ bIn :=
+      fix rect b Γ bIn {struct Γ} : P b Γ bIn :=
+        In_case _ fz (fun _ _ _ bIn => fs _ _ _ bIn (rect _ _ bIn)) bIn.
+
+    Definition In_ind (P : forall b Γ, In b Γ -> Prop)
+      (fz : forall b Γ, P b (snoc Γ b) in_zero)
+      (fs : forall b Γ b' bIn, P b Γ bIn -> P b (snoc Γ b') (in_succ bIn)) :
+      forall b Γ bIn, P b Γ bIn :=
+      In_rect P fz fs.
+
+    (* A small tactic used locally to reduce an eta-expanded [In] record. The
+       eta-expansion happens quite frequently. For instance, the smart
+       constructors [in_zero] and [in_succ] are implemented by pattern
+       matching on a record, which therefore will need eta-reduction after
+       simplification. *)
+    #[local] Ltac in_eta_reduce :=
+      repeat
+        match goal with
+        | H: context[{| in_at := in_at ?x; in_valid := in_valid ?x |}] |- _ =>
+            change_no_check {| in_at := in_at x; in_valid := in_valid x |} with x in H
+        | |- context[{| in_at := in_at ?x; in_valid := in_valid ?x |}] =>
+            change_no_check {| in_at := in_at ?x; in_valid := in_valid ?x |} with x
+        end.
+
+    (* We define several views on [In] which allows us to define mechanisms for
+       reusable dependent pattern matching. For more information on views as a
+       programming technique see:
+       - Ulf Norell (2009), "Dependently Typed Programming in Agda." AFP'08.
+         https://doi.org/10.1007/978-3-642-04652-0_5
+       - Philip Wadler (1987). "Views: a way for pattern matching to cohabit
+         with data abstraction." POPL'87.
+         https://doi.org/10.1145/41625.41653
+       - Conor McBride & James McKinna (2004). "The view from the left." JFP'04.
+         https://doi.org/10.1017/S0956796803004829 *)
+
+    (* A view expressing that membership in the empty context is uninhabited. *)
+    Variant NilView [b : B] (i : In b nil) : Type :=.
+
+    (* A view for membership in a non-empty context. *)
+    Variant SnocView {b' : B} (Γ : Ctx B) :
+      forall b, In b (snoc Γ b') -> Type :=
+    | isZero                  : SnocView in_zero
+    | isSucc {b} (i : In b Γ) : SnocView (in_succ i).
+    #[global] Arguments SnocView {_ _} [b] _.
+    #[global] Arguments isZero {_ _}.
+
+    (* Instead of defining separate view functions, that construct a value
+       of the *View datatypes, we use a single definition. This way, we
+       avoid definition dummy definitions the other cases like it is usually
+       done in small inversions. We simply define inversions for all cases at
+       once. *)
+    Definition view : forall {b Γ} (bIn : In b Γ),
+        match Γ return forall b, In b Γ -> Type with
+        | nil      => NilView
+        | snoc _ _ => SnocView
+        end b bIn :=
+      In_case _ (@isZero) (@isSucc).
+
+    (* Left and right membership proofs for context concatenation. *)
+    Fixpoint in_cat_left {b Γ} Δ (bIn : In b Γ) : In b (cat Γ Δ) :=
+      match Δ with
+      | nil      => bIn
+      | snoc Δ _ => in_succ (in_cat_left Δ bIn)
+      end.
+
+    Fixpoint in_cat_right {b Γ} Δ (bIn : In b Δ) : In b (cat Γ Δ) :=
+      In_case (fun b Δ _ => In b (cat Γ Δ))
+        (fun _ Δ => @in_zero _ (cat Γ Δ))
+        (fun _ _ _ i => in_succ (in_cat_right i)) bIn.
+
+    (* A view for case splitting on a proof of membership in a concatenation.
+       By pattern matching on this view we get the membership in the left
+       respectively right side of the concatenation and refine the original
+       membership proof. *)
+    Inductive CatView {Γ Δ} [b : B] : In b (cat Γ Δ) -> Type :=
+    | isCatLeft  (bIn : In b Γ) : CatView (in_cat_left Δ bIn)
+    | isCatRight (bIn : In b Δ) : CatView (in_cat_right bIn).
+
+    (* The view functions that constructs a concatenation view. *)
+    Fixpoint catView {Γ Δ} : forall b (bIn : In b (cat Γ Δ)), CatView bIn :=
+      match Δ with
+      | nil       => isCatLeft
+      | snoc Δ b' =>
+          fun b bIn =>
+            match view bIn with
+            | isZero   => isCatRight in_zero
+            | isSucc bIn =>
+                match catView bIn with
+                | isCatLeft  bIn => isCatLeft bIn
+                | isCatRight bIn => isCatRight (in_succ bIn)
+                end
+            end
+      end.
+
+    #[program] Instance NoConfusionPackage_In {uip_B : UIP B} {b Γ} :
+      NoConfusionPackage (In b Γ) :=
+      {| NoConfusion xIn yIn := NoConfusion (in_at xIn) (in_at yIn);
+         noConfusion xIn yIn (e : NoConfusion (in_at xIn) (in_at yIn)) :=
+           match noConfusion e in _ = y
+           return forall q, xIn = {| in_at := y; in_valid := q |}
+           with
+           | eq_refl => fun q => f_equal (MkIn _) (proof_irrelevance_nth_is _ _ (in_valid xIn) q)
+           end (in_valid yIn);
+         noConfusion_inv (xIn yIn : In b Γ) (e : xIn = yIn) :=
+           noConfusion_inv (f_equal (@in_at b Γ) e);
+      |}.
+    Next Obligation.
+      intros ? ? ? [m p] [n q] e. cbn [in_at in_valid] in *.
+      etransitivity; [|apply noConfusion_sect].
+      now destruct (noConfusion e), (proof_irrelevance_nth_is m b p q).
+    Qed.
+    Next Obligation.
+      intros ? ? ? [m p] [n q] e; intros.
+      destruct e.
+      destruct Γ; cbn in *. contradiction.
+      destruct m, n.
+      - destruct p. cbn. now rewrite EqDec.uip_refl_refl.
+      - destruct p. cbn. now rewrite EqDec.uip_refl_refl.
+      - cbn. rewrite proof_irrelevance_nth_is_refl. reflexivity.
+      - cbn. rewrite proof_irrelevance_nth_is_refl. reflexivity.
+    Qed.
+
+    (* Two proofs of context membership are equal of the deBruijn indices are equal *)
     Definition In_eqb {Γ} {b1 b2 : B} (b1inΓ : In b1 Γ) (b2inΓ : In b2 Γ) : bool :=
       Nat.eqb (in_at b1inΓ) (in_at b2inΓ).
 
@@ -225,120 +356,6 @@ Module Import ctx.
         now dependent elimination Heq.
       - intros e. depelim e. destruct n, m; cbn in H; congruence.
     Qed.
-
-    (* These are *constructors* for In. *)
-    Definition in_zero {b : B} {Γ : Ctx B} : In b (snoc Γ b) :=
-      @MkIn _ (snoc Γ b) 0 eq_refl.
-    Definition in_succ {b : B} {Γ : Ctx B} {b' : B} (bIn : In b Γ) :
-      In b (snoc Γ b') :=
-      @MkIn _ (snoc Γ b') (S (in_at bIn)) (in_valid bIn).
-
-    Inductive NilView {b : B} (i : In b nil) : Type :=.
-
-    Definition nilView {b : B} (i : In b nil) : NilView i :=
-      match in_valid i with end.
-
-    Inductive SnocView (Γ : Ctx B) {b' : B} : forall b, In b (snoc Γ b') -> Type :=
-    | snocViewZero                  : SnocView in_zero
-    | snocViewSucc {b} (i : In b Γ) : SnocView (in_succ i).
-    Global Arguments snocViewZero {_ _}.
-
-    Definition snocView {Γ} {b b' : B} (i : In b (snoc Γ b')) :
-      @SnocView Γ b' b i :=
-      match in_at i as n return forall p, SnocView (MkIn n p)
-      with
-      | O   => fun p => match p with eq_refl => snocViewZero end
-      | S n => fun p => snocViewSucc (MkIn n p)
-      end (in_valid i).
-
-    Inductive InView {b : B} : forall Γ, In b Γ -> Type :=
-    | inctxViewZero {Γ}                 : @InView b (snoc Γ b) in_zero
-    | inctxViewSucc {Γ b'} (i : In b Γ) : @InView b (snoc Γ b') (in_succ i).
-
-    Definition inView {b Γ} : forall bIn : In b Γ, InView bIn :=
-      match Γ with
-      | nil      => fun bIn => match nilView bIn with end
-      | snoc Γ b => fun bIn =>
-        match snocView bIn with
-        | snocViewZero   => inctxViewZero
-        | snocViewSucc i => inctxViewSucc i
-        end
-      end.
-
-    Fixpoint in_cat_left {b : B} {Γ : Ctx B} (Δ : Ctx B) (bIn : In b Γ) : In b (cat Γ Δ) :=
-      match Δ with
-      | nil      => bIn
-      | snoc Δ _ => in_succ (in_cat_left Δ bIn)
-      end.
-
-    Fixpoint in_cat_right {b : B} {Γ : Ctx B} (Δ : Ctx B) : In b Δ -> In b (cat Γ Δ) :=
-      match Δ with
-      | nil      => fun bIn => match nilView bIn with end
-      | snoc _ _ =>
-        fun bIn =>
-          match snocView bIn with
-          | snocViewZero => @in_zero _ (cat _ _)
-          | snocViewSucc bIn => in_succ (in_cat_right bIn)
-          end
-      end.
-
-    Inductive CatView {Γ Δ} {b : B} : In b (cat Γ Δ) -> Type :=
-    | isCatLeft  (bIn : In b Γ) : CatView (in_cat_left Δ bIn)
-    | isCatRight (bIn : In b Δ) : CatView (in_cat_right bIn).
-
-    Definition catView_succ {Γ Δ b b'} (bIn : In b (cat Γ Δ)) (bInV : CatView bIn) :
-      @CatView Γ (snoc Δ b') b (in_succ bIn) :=
-      match bInV with
-      | isCatLeft bIn => @isCatLeft Γ (@snoc B Δ b') b bIn
-      | isCatRight bIn => @isCatRight Γ (@snoc B Δ b') b (@in_succ b Δ b' bIn)
-      end.
-
-    Fixpoint catView_index {Γ Δ} {b : B} {struct Δ} :
-      forall (n : nat) (p : nth_is (cat Γ Δ) n b),
-        @CatView Γ Δ b (@MkIn b (cat Γ Δ) n p) :=
-      match Δ with
-      | nil => fun n p => @isCatLeft Γ (@nil B) b (@MkIn b Γ n p)
-      | snoc Δ0 b0 =>
-        fun n =>
-          match n with
-          | 0 =>
-            fun p =>
-              match
-                p as e in (_ = y)
-                return (@CatView Γ (@snoc B Δ0 b0) y (@MkIn y (@snoc B (cat Γ Δ0) b0) 0 e))
-              with
-              | eq_refl => @isCatRight Γ (@snoc B Δ0 b0) b0 (@in_zero b0 Δ0)
-              end
-          | S n => fun p => catView_succ (catView_index n p)
-          end
-      end.
-
-    Definition catView {Γ Δ} {b : B} (bIn : In b (cat Γ Δ)) : CatView bIn :=
-      @catView_index Γ Δ b (@in_at _ _ bIn) (@in_valid _ _ bIn).
-
-    Definition In_rect (b : B)
-      (P : forall (Γ : Ctx B), In b Γ -> Type)
-      (fzero : forall (Γ : Ctx B), P (snoc Γ b) in_zero)
-      (fsucc : forall (Γ : Ctx B) (b0 : B) (bIn : In b Γ),
-          P Γ bIn -> P (snoc Γ b0) (in_succ bIn)) :
-      forall (Γ : Ctx B) (bIn : In b Γ), P Γ bIn.
-    Proof.
-      induction Γ; cbn.
-      - intro bIn. destruct (nilView bIn).
-      - intros bIn. destruct (snocView bIn).
-        + apply fzero.
-        + now apply fsucc.
-    Defined.
-    Global Arguments In_rect [_] _.
-
-    Definition In_ind (b : B)
-      (P : forall (Γ : Ctx B), In b Γ -> Prop)
-      (fzero : forall (Γ : Ctx B), P (snoc Γ b) in_zero)
-      (fsucc : forall (Γ : Ctx B) (b0 : B) (bIn : In b Γ),
-          P Γ bIn -> P (snoc Γ b0) (in_succ bIn)) :
-      forall (Γ : Ctx B) (bIn : In b Γ), P Γ bIn :=
-      In_rect P fzero fsucc.
-    Global Arguments In_ind [_] _.
 
     Section All.
 
@@ -355,67 +372,26 @@ Module Import ctx.
 
     End All.
 
-    Fixpoint remove (Γ : Ctx B) {b : B} : In b Γ -> Ctx B :=
-      match Γ with
-      | nil =>
-        fun '(MkIn n e) =>
-          match e with end
-      | snoc Γ b' =>
-        fun '(MkIn n e) =>
-          match n return (nth_is (snoc Γ b') n b -> Ctx B)
-          with
-          | 0   => fun _ => Γ
-          | S n => fun e  => snoc (@remove Γ b (MkIn n e)) b'
-          end e
-      end.
+    Fixpoint remove (Γ : Ctx B) {b} (bIn : In b Γ) {struct Γ} : Ctx B :=
+      In_case _ (fun _ Γ => Γ) (fun b' _ _ bIn => snoc (remove bIn) b') bIn.
     Arguments remove _ [_] _.
 
-    Fixpoint shift_index {b x} {Σ : Ctx B} {struct Σ} :
-      forall
-        (bn xn : nat) (bp : nth_is Σ bn b)
-        (xp : nth_is (remove Σ {| in_valid := bp |}) xn x),
-        In x Σ :=
-      match Σ with
-      | nil => fun _ _ (bp : nth_is nil _ _) => match bp with end
-      | snoc Σ b =>
-        fun bn xn =>
-          match bn , xn with
-          | O    , xn   => fun bp xp => in_succ (MkIn xn xp)
-          | S bn , O    => fun bp xp => MkIn (Γ := snoc Σ b) O xp
-          | S bn , S xn => fun bp xp => in_succ (shift_index bn xn bp xp)
-          end
-      end.
+    Fixpoint shift_var {b x Γ} (bIn : In b Γ) {struct Γ} :
+      In x (remove Γ bIn) -> In x Γ :=
+      In_case
+        (fun _ Γ xIn => In x (remove Γ xIn) -> In x Γ)
+        (fun _ _ xIn => in_succ xIn)
+        (fun b' Γ b bIn (xIn : In x (snoc (remove Γ bIn) b')) =>
+           match view xIn with
+           | isZero     => in_zero
+           | isSucc xIn => in_succ (shift_var bIn xIn)
+           end) bIn.
 
-    Definition shift_var {b x} {Σ : Ctx B} (bIn : In b Σ) (xIn : In x (remove Σ bIn)) : In x Σ :=
-      shift_index (in_at bIn) (in_at xIn) (in_valid bIn) (in_valid xIn).
-
-    (* Most explicit type-signatures given below are only necessary for Coq 8.9
-       and can be cleaned up for later versions. *)
-    Fixpoint occurs_check_index {Σ} {x y : B} (m n : nat) {struct Σ} :
-      forall (p : nth_is Σ m x) (q : nth_is Σ n y),
-        (x = y) + (In y (remove _ {| in_at := m; in_valid := p |})) :=
-      match Σ with
-      | nil => fun _ (q : nth_is nil n y) => match q with end
-      | snoc Σ b =>
-        match m , n with
-        | 0   , 0   => fun (p : nth_is (snoc Σ b) 0 x) q =>
-                         inl (eq_trans (eq_sym p) q)
-        | 0   , S n => fun p (q : nth_is (snoc Σ b) (S n) y) =>
-                         inr (@MkIn _ (remove _ (@MkIn _ (snoc Σ b) 0 p)) n q)
-        | S m , 0   => fun _ (q : nth_is (snoc Σ b) 0 y) =>
-                         inr (@MkIn _ (snoc (remove Σ _) b) 0 q)
-        | S m , S n => fun p q => base.sum_map id in_succ (occurs_check_index m n p q)
-        end
-      end.
-
-    Definition occurs_check_var {Σ} {x y : B} (xIn : In x Σ) (yIn : In y Σ) : (x = y) + (In y (remove Σ xIn)) :=
-      occurs_check_index (in_at xIn) (in_at yIn) (in_valid xIn) (in_valid yIn).
-
-    Inductive OccursCheckView {Σ} {x : B} (xIn : In x Σ) : forall y, In y Σ -> Type :=
+    Inductive OccursCheckView {Σ x} (xIn : In x Σ) : forall y, In y Σ -> Type :=
     | Same : OccursCheckView xIn xIn
     | Diff {y} (yIn : In y (remove Σ xIn)) : OccursCheckView xIn (shift_var xIn yIn).
 
-    Definition occurs_check_view_step {Σ} {b x y: B} (xIn : In x Σ) (yIn : In y Σ) :
+    Definition occurs_check_view_step {Σ b x y} (xIn : In x Σ) (yIn : In y Σ) :
       OccursCheckView xIn yIn ->
       OccursCheckView (Σ := snoc Σ b) (in_succ xIn) (in_succ yIn) :=
       fun v =>
@@ -424,96 +400,31 @@ Module Import ctx.
       | Diff _ yIn => Diff (in_succ xIn) (in_succ yIn)
       end.
 
-    Fixpoint occurs_check_view_index {Σ} {x y: B} {m n : nat} {struct Σ} :
-      forall (p : nth_is Σ m x) (q : nth_is Σ n y),
-        OccursCheckView
-          {| in_at := m; in_valid := p |}
-          {| in_at := n; in_valid := q |} :=
-      match Σ with
-      | nil => fun _ (q : nth_is nil n y) => match q with end
-      | snoc Σ b =>
-        match m , n with
-        | 0   , 0   => fun (p : nth_is (snoc Σ b) 0 x) q =>
-                         match p , q with
-                         | eq_refl , eq_refl =>
-                             Same (@MkIn b (@snoc B Σ b) 0 eq_refl)
-                         end
-        | 0   , S n => fun p (q : nth_is (snoc Σ b) (S n) y) =>
-                         Diff
-                           (@MkIn x (@snoc B Σ b) 0 p)
-                           (@MkIn y Σ n q)
-        | S m , 0   => fun p (q : nth_is (snoc Σ b) 0 y) =>
-                         Diff
-                           (@MkIn x (@snoc B Σ b) (S m) p)
-                           (@MkIn _ (snoc (remove Σ _) b) 0 q)
-        | S m , S n => fun p q =>
-                         occurs_check_view_step
-                           (@occurs_check_view_index Σ x y m n p q)
-        end
-      end.
+    Fixpoint occurs_check_view {Γ x} (xIn : In x Γ) :
+      forall {y} (yIn : In y Γ), OccursCheckView xIn yIn :=
+      In_case
+        (fun x Γ xIn => forall y (yIn : In y Γ), OccursCheckView xIn yIn)
+        (fun x Γ y (yIn : In y (snoc Γ x)) =>
+           match view yIn with
+           | isZero     => Same in_zero
+           | isSucc yIn => Diff in_zero yIn
+           end)
+        (fun z Γ x (xIn : In x Γ) y (yIn : In y (snoc Γ z)) =>
+           match view yIn with
+           | isZero     => Diff (in_succ xIn) in_zero
+           | isSucc yIn => occurs_check_view_step (occurs_check_view xIn yIn)
+           end) xIn.
 
-    Definition occurs_check_view {Σ} {x y: B} (xIn : In x Σ) (yIn : In y Σ) : OccursCheckView xIn yIn :=
-      occurs_check_view_index (in_valid xIn) (in_valid yIn).
-
-    Lemma occurs_check_view_refl {Σ x} (xIn : In x Σ) :
+    Lemma occurs_check_view_refl {Γ x} (xIn : In x Γ) :
       occurs_check_view xIn xIn = Same _.
-    Proof.
-      unfold occurs_check_view.
-      induction xIn using In_ind.
-      - reflexivity.
-      - cbn; now rewrite IHxIn.
-    Qed.
+    Proof. induction xIn using In_ind; cbn; in_eta_reduce; now rewrite ?IHxIn. Qed.
 
     Lemma occurs_check_view_shift {Σ x y} (xIn : In x Σ) (yIn : In y (remove Σ xIn)) :
       occurs_check_view xIn (shift_var xIn yIn) = Diff xIn yIn.
     Proof.
-      unfold occurs_check_view, shift_var.
-      induction xIn using In_ind.
-      - reflexivity.
-      - cbn in yIn. destruct (snocView yIn); cbn.
-        + reflexivity.
-        + now rewrite (IHxIn i).
-    Qed.
-
-    Lemma occurs_check_var_spec {Σ} {x y : B} (xIn : In x Σ) (yIn : In y Σ) :
-      match occurs_check_var xIn yIn with
-      | inl e    => eq_rect x (fun z => In z Σ) xIn y e = yIn
-      | inr yIn' => yIn = shift_var xIn yIn' /\ in_at xIn <> in_at yIn
-      end%type.
-    Proof.
-      unfold occurs_check_var, shift_var; destruct yIn as [n q]; revert n q.
-      induction xIn using In_ind; intros n q.
-      - destruct n.
-        + now destruct q.
-        + split. reflexivity. cbn. intuition.
-      - destruct n; cbn.
-        + split. reflexivity. intuition.
-        + specialize (IHxIn n q); revert IHxIn; cbn.
-          destruct (occurs_check_index (in_at xIn) n (in_valid xIn) q).
-          * destruct e; cbn. now intros ->.
-          * destruct xIn as [m p]; cbn. intros [<- ?]. intuition.
-    Qed.
-
-    Lemma occurs_check_var_refl {Σ x} (xIn : In x Σ) :
-      occurs_check_var xIn xIn = inl eq_refl.
-    Proof.
-      unfold occurs_check_var.
-      induction xIn using In_ind.
-      - reflexivity.
-      - cbn; now rewrite IHxIn.
-    Qed.
-
-    Lemma occurs_check_shift_var {Σ x y} (xIn : In x Σ) (yIn : In y (remove Σ xIn)) :
-      occurs_check_var xIn (shift_var xIn yIn) = inr yIn.
-    Proof.
-      unfold occurs_check_var, shift_var. destruct yIn as [m p]. cbn.
-      revert m p.
-      induction xIn using In_ind.
-      - reflexivity.
-      - intros [|m]; cbn.
-        + reflexivity.
-        + intros p.
-          now rewrite (IHxIn m p).
+      induction xIn using In_ind; [easy|].
+      change_no_check (In y (snoc (remove Γ xIn) b')) in yIn.
+      destruct (view yIn); [easy|]. cbn. in_eta_reduce. now rewrite IHxIn.
     Qed.
 
     Local Open Scope lazy_bool_scope.
@@ -524,47 +435,33 @@ Module Import ctx.
       | snoc Γ b => fun p => p b in_zero &&& forallb (fun b bIn => p b (in_succ bIn))
       end.
 
-    Fixpoint flip_remove_index {Γ : Ctx B} {y x} (n m : nat) {struct Γ} :
-      forall
-        (q : nth_is Γ n y)
-        (p : nth_is (remove Γ {| in_at := n; in_valid := q |}) m x),
-        In y (remove Γ (shift_index n m q p)) :=
-     match Γ with
-     | nil => fun q => match q with end
-     | snoc Γ b =>
-         match n with
-         | 0 =>
-           fun q p =>
-             @MkIn y (remove (snoc Γ b) (shift_index 0 m q p)) 0 q
-         | S n =>
-           fun q =>
-             match m with
-             | 0 => fun _ => @MkIn y Γ n q
-             | S m => fun p => in_succ (flip_remove_index n m q p)
-             end
-         end
-     end.
-
     (* Calculates x ∈ Γ - y => y ∈ Γ - x *)
-    Definition flip_remove {Γ : Ctx B} {y x : B} (yIn : In y Γ) (xIn : In x (@remove Γ y yIn)) :
-      In y (@remove Γ x (@shift_var y x Γ yIn xIn)) :=
-      flip_remove_index (in_at yIn) (in_at xIn) (in_valid yIn) (in_valid xIn).
+    Fixpoint flip_remove {Γ y} (yIn : In y Γ) :
+      forall {x} (xIn : In x (remove Γ yIn)),
+        In y (remove Γ (shift_var yIn xIn)) :=
+      In_case
+        (fun y Γ yIn =>
+           forall x (xIn : In x (remove Γ yIn)),
+             In y (remove Γ (shift_var yIn xIn)))
+        (fun _ _ _ _ => in_zero)
+        (fun b' Γ y yIn x (xIn : In x (snoc (remove Γ yIn) b')) =>
+           match view xIn in SnocView xIn
+           return In y (remove (snoc Γ b') (shift_var (in_succ yIn) xIn))
+           with
+           | isZero     => yIn
+           | isSucc xIn => in_succ (flip_remove yIn xIn)
+           end) yIn.
 
     (* Σ - y - x = Σ - x - y *)
-    Lemma swap_remove {Γ : Ctx B} {y x} (yIn : In y Γ) (xIn : In x (remove Γ yIn)) :
-      remove (remove Γ yIn) xIn =
-      remove (remove Γ (shift_var yIn xIn)) (flip_remove yIn xIn).
+    Lemma swap_remove {Γ : Ctx B} {y} (yIn : In y Γ) :
+      forall x (xIn : In x (remove Γ yIn)),
+        remove (remove Γ yIn) xIn =
+        remove (remove Γ (shift_var yIn xIn)) (flip_remove yIn xIn).
     Proof.
-      destruct yIn as [n q], xIn as [m p]. cbn in *.
-      unfold shift_var. cbn.
-      revert n q m p.
-      induction Γ; intros n q m p.
-      destruct q.
-      destruct n; cbn in q.
-      - reflexivity.
-      - destruct m; cbn in p.
-        + reflexivity.
-        + cbn in *. f_equal. apply IHΓ.
+      induction yIn using In_ind; [easy|].
+      change_no_check (remove (snoc ?Γ ?b) (in_succ ?xIn))
+        with (snoc (remove Γ xIn) b).
+      intros x xIn; destruct (view xIn); cbn; in_eta_reduce; now f_equal.
     Defined.
 
     Definition f_equal_snoc (b : B) Γ Δ (e : Γ = Δ) : snoc Γ b = snoc Δ b :=
@@ -580,33 +477,25 @@ Module Import ctx.
       eq_rect x (fun x => Q (snoc x b)) z y e :=
       map_subst_map (fun Γ => snoc Γ b) (fun _ x => x) e z.
 
-    Fixpoint remove_in_cat_right (Γ Δ : Ctx B) {struct Δ} :
-      forall b (bIn : In b Δ),
-        remove (cat Γ Δ) (in_cat_right bIn) =
-          cat Γ (remove Δ bIn) :=
-      match Δ with
-      | nil        => fun b bIn => match nilView bIn with end
-      | snoc Δ' b' =>
-        fun b bIn =>
-          match snocView bIn in SnocView i
-          return remove _ (in_cat_right i) = cat Γ (remove _ i)
-          with
-          | snocViewZero   => eq_refl
-          | snocViewSucc i => f_equal_snoc b' (remove_in_cat_right _ i)
-          end
-      end.
+    Fixpoint remove_in_cat_right (Γ Δ : Ctx B) {b} (bIn : In b Δ) :
+      remove (cat Γ Δ) (in_cat_right bIn) = cat Γ (remove Δ bIn) :=
+      In_case
+        (fun b Δ bIn => remove (cat Γ Δ) (in_cat_right bIn) = cat Γ (remove Δ bIn))
+        (fun _ _        => eq_refl)
+        (fun b' Δ b bIn => f_equal_snoc b' (remove_in_cat_right _ bIn))
+        bIn.
 
     Fixpoint remove_in_cat_left (Γ Δ : Ctx B) {b} (bIn : In b Γ) {struct Δ} :
-      remove (cat Γ Δ) (in_cat_left Δ bIn) =
-        cat (remove Γ bIn) Δ :=
+      remove (cat Γ Δ) (in_cat_left Δ bIn) = cat (remove Γ bIn) Δ :=
       match Δ with
       | nil        => eq_refl
       | snoc Δ' b' => f_equal_snoc b' (remove_in_cat_left _ bIn)
       end.
 
   End WithBinding.
-  Arguments In_rect [B b] _ _ _ [_] : simpl never.
-  Arguments In_ind [B b] _ _ _ [_] : simpl never.
+  Arguments In_case [B] P fz fs [b Γ] i.
+  Arguments In_rect [B] P fz fs [b Γ] : simpl never.
+  Arguments In_ind [B] P fz fs [b Γ] : simpl never.
   Arguments forallb [B] Γ p.
   Arguments remove_in_cat_right [B Γ Δ b] bIn.
   Arguments remove_in_cat_left [B Γ Δ b] bIn.
@@ -622,11 +511,10 @@ Module Import ctx.
 
     (* This is proof relevant because it's used in the automatic translation
        of program variables to logic variables. *)
-    Definition in_map {a : A} : forall Γ, In a Γ -> In (f a) (map Γ) :=
-      In_rect
-        (fun Γ _ => In (f a) (map Γ))
-        (fun Γ   => in_zero)
-        (fun Γ _ _ => in_succ).
+    Definition in_map : forall a Γ, In a Γ -> In (f a) (map Γ) :=
+      In_rect (fun a Γ _ => In (f a) (map Γ))
+        (fun _ _       => in_zero)
+        (fun _ _ _ _ i => in_succ i).
 
   End WithAB.
 
